src/cnf/Cnf.v
@@ -305,8 +305,19 @@ Section CHECKER.
     | _ => C._true
     end.
 
+  Definition check_NotSimplify l := 
+    match get_hash (Lit.blit l) with
+    | Fiff a b => 
+        match get_hash (Lit.blit a), get_hash (Lit.blit a) with
+        | Fnot2 1 x, _ => if x == b then (l::nil) else C._true
+        | Ffalse, Ftrue => if negb (Lit.is_pos a) then (l::nil) else C._true
+        | Ftrue, Ffalse => if negb (Lit.is_pos a) then (l::nil) else C._true
+        | _, _ => C._true
+        end
+    | _ => C._true
+    end.
 
-
+    
   (** The correctness proofs *)
 
   Variable interp_atom : atom -> bool.
@@ -431,6 +442,11 @@ Section CHECKER.
            - now rewrite Lit.interp_neg, Hi.
          }
   Qed.
+  
+  Lemma valid_check_NotSimplify : forall l, C.valid rho (check_NotSimplify l).
+  Proof.
+    admit.
+  Admitted.
 
   Hypothesis Hs : S.valid rho s.
 
